syn/ex/Mesi/MesiComp.v
@@ -1,0 +1,30 @@
+Require Import String.
+
+Require Import Compiler.Compiler.
+Require Import MesiDeep.
+
+Set Implicit Arguments.
+
+Section Tests.
+
+  Definition oidx: IdxT := 1.
+  Definition uln: string := "UpLock". 
+  Definition dln: string := "DownLock".
+  Definition ostin: string := "ost".
+
+  Context `{cet: @CompExtType DirExtType}
+          `{@CompExtExp SpecInds.NatDecValue
+                        Mesi.ImplOStateIfc
+                        mesiHConfig
+                        DirExtType
+                        DirExtExp
+                        cet}.
+
+  Existing Instance MesiHOStateIfcFull.
+  Definition cl1GetSImm := compile_Rule oidx uln dln ostin (existT _ _ (hl1GetSImm oidx)).
+  Goal True.
+    pose cl1GetSImm as r.
+    compute in r.
+  Abort.
+
+End Tests.
