syn/ex/Mesi/MesiDeep.v
@@ -1,0 +1,232 @@
+Require Import Compiler.Compiler.
+
+Require Import Hemiola.Common Hemiola.Index Hemiola.HVector.
+Require Import Hemiola.Ex.TopoTemplate Hemiola.Ex.RuleTemplate.
+Require Import Hemiola.Ex.Mesi.Mesi.
+
+Require Import FunctionalExtensionality.
+
+Set Implicit Arguments.
+
+Section Tests.
+
+  Lemma abcd: forall A B C D, (A <-> B) -> (C <-> D) -> (A /\ C <-> B /\ D).
+  Proof. firstorder. Qed.
+
+  Lemma TrsMTrs_ext:
+    forall `{DecValue} `{OStateIfc} (trs1 trs2: StateMTrs),
+      (forall stm, trs1 stm = trs2 stm) ->
+      forall ost orq mins,
+        TrsMTrs trs1 ost orq mins = TrsMTrs trs2 ost orq mins.
+  Proof.
+    cbv [TrsMTrs]; intros.
+    rewrite H1; reflexivity.
+  Qed.
+
+  Variable oidx: IdxT.
+
+  Instance mesiHConfig: hconfig :=
+    {| hcfg_oidx_sz := (2, 3);
+       hcfg_midx_sz := (4, 4);
+       hcfg_msg_id_sz := (3, 2);
+       hcfg_value_sz := 32;
+       hcfg_children_max_lg := 2;
+    |}.
+
+  Existing Instance SpecInds.NatDecValue.
+  Existing Instance Mesi.ImplOStateIfc.
+
+  Definition HMesi := HNat 3.
+
+  Lemma MesiHOStateIfc_host_ty_ok:
+    forall i: Fin.t ost_sz,
+      match Vector.nth [Some HValue; Some HBool; Some HMesi; None]%vector i with
+      | Some hbt => Vector.nth ost_ty i = hbtypeDenote hbt
+      | None => True
+      end.
+  Proof.
+    intros.
+    refine (match i with | Fin.F1 => _ | Fin.FS _ => _ end);
+      [repeat (destruct n; [exact idProp|]);
+       destruct n; [|exact idProp];
+       reflexivity
+      |repeat (destruct n; [exact idProp|]);
+       destruct n; [|exact idProp]].
+    refine (match t with | Fin.F1 => _ | Fin.FS _ => _ end);
+      [repeat (destruct n; [exact idProp|]);
+       destruct n; [|exact idProp];
+       reflexivity
+      |repeat (destruct n; [exact idProp|]);
+       destruct n; [|exact idProp]].
+    refine (match t0 with | Fin.F1 => _ | Fin.FS _ => _ end);
+      [repeat (destruct n; [exact idProp|]);
+       destruct n; [|exact idProp];
+       reflexivity
+      |repeat (destruct n; [exact idProp|]);
+       destruct n; [|exact idProp]].
+    refine (match t1 with | Fin.F1 => _ | Fin.FS _ => _ end);
+      [repeat (destruct n; [exact idProp|]);
+       destruct n; [|exact idProp];
+       reflexivity
+      |repeat (destruct n; [exact idProp|]);
+       destruct n; [|exact idProp]].
+    apply Fin.case0; assumption.
+  Defined.
+
+  Instance MesiHOStateIfc: HOStateIfc :=
+    {| host_ty := [Some HValue; Some HBool; Some HMesi; None]%vector;
+       host_ty_ok := MesiHOStateIfc_host_ty_ok;
+    |}.
+
+  Section DirExt.
+
+    Inductive htype_dir: Set :=
+    | HDir: htype_dir.
+
+    Definition htypeDenote_dir (ht: htype_dir): Type :=
+      match ht with
+      | HDir => Mesi.DirT
+      end.
+
+    Instance DirExtType: ExtType :=
+      {| hetype := htype_dir;
+         hetypeDenote := htypeDenote_dir
+      |}.
+
+    Inductive hexp_dir (var: htype -> Type): htype -> Type :=
+    | HDirC: hexp_dir var (HEType HDir)
+    | HDirGet: hbexp (bvar var) HIdxO ->
+               hexp_dir var (HEType HDir) ->
+               hexp_dir var (HBType (HNat 3)).
+
+    Fixpoint interp_hexp_dir (ost: OState) (orq: ORq Msg) (mins: list (Id Msg))
+             {ht} (he: hexp_dir htypeDenote ht): htypeDenote ht :=
+      match he in (hexp_dir _ h) return (htypeDenote h) with
+      | HDirC _ => (ost#[dir])%hvec
+      | HDirGet oidx dir => getDir (interpBExp ost oidx) (interp_hexp_dir ost orq mins dir)
+      end.
+
+    Instance DirExtExp: ExtExp :=
+      {| heexp := hexp_dir;
+         interp_heexp := interp_hexp_dir
+      |}.
+
+  End DirExt.
+
+  Existing Instance DirExtType.
+  Existing Instance DirExtExp.
+
+  Lemma MesiHOStateIfcFull_hostf_ty_compat:
+    forall i hbt,
+      host_ty[@i] = Some hbt ->
+      [HBType HValue; HBType HBool; HBType HMesi; HEType HDir][@i] = HBType hbt.
+  Proof.
+    intros i.
+    refine (match i with | Fin.F1 => _ | Fin.FS _ => _ end);
+      [repeat (destruct n; [exact idProp|]);
+       destruct n; [|exact idProp];
+       simpl; intros; congruence
+      |repeat (destruct n; [exact idProp|]);
+       destruct n; [|exact idProp]].
+    refine (match t with | Fin.F1 => _ | Fin.FS _ => _ end);
+      [repeat (destruct n; [exact idProp|]);
+       destruct n; [|exact idProp];
+       simpl; intros; congruence
+      |repeat (destruct n; [exact idProp|]);
+       destruct n; [|exact idProp]].
+    refine (match t0 with | Fin.F1 => _ | Fin.FS _ => _ end);
+      [repeat (destruct n; [exact idProp|]);
+       destruct n; [|exact idProp];
+       simpl; intros; congruence
+      |repeat (destruct n; [exact idProp|]);
+       destruct n; [|exact idProp]].
+    refine (match t1 with | Fin.F1 => _ | Fin.FS _ => _ end);
+      [repeat (destruct n; [exact idProp|]);
+       destruct n; [|exact idProp];
+       simpl; intros; congruence
+      |repeat (destruct n; [exact idProp|]);
+       destruct n; [|exact idProp]].
+    apply Fin.case0; assumption.
+  Defined.
+
+  Instance MesiHOStateIfcFull: HOStateIfcFull :=
+    {| hostf_ty := [HBType HValue; HBType HBool; HBType HMesi; HEType HDir];
+       hostf_ty_ok := eq_refl;
+       hostf_ty_compat := MesiHOStateIfcFull_hostf_ty_compat;
+    |}.
+  
+  Definition hl1GetSImm: HRule (l1GetSImm (l1ExtOf oidx)).
+  Proof.
+    refine {| hrule_msg_from := _ |}.
+
+    - intros.
+      repeat autounfold with MesiRules.
+      cbv [immDownRule].
+      cbv [rule_precond].
+
+      apply abcd.
+
+      + cbv [interpMsgFrom].
+        instantiate (1:= HMsgFromExt _).
+        apply iff_refl.
+
+      + instantiate (1:= fun var => HOPrecAnd (var:= var) _ _); simpl; apply abcd.
+        all: repeat
+               match goal with
+               | |- _ <-> (_ /\oprec _) _ _ _ =>
+                 instantiate (1:= HOPrecAnd _ _); simpl; apply abcd
+               end.
+
+        1-4: instantiate (1:= HOPrecRqRs _ _); simpl.
+        1-4: first [instantiate (1:= HRqAccepting); apply iff_refl; fail
+                   |instantiate (1:= HRsAccepting); apply iff_refl; fail
+                   |instantiate (1:= HUpLockFree); apply iff_refl; fail
+                   |instantiate (1:= HDownLockFree); apply iff_refl; fail
+                   |instantiate (1:= HUpLockMsgId _ _); apply iff_refl; fail
+                   |instantiate (1:= HUpLockMsg); apply iff_refl; fail
+                   |instantiate (1:= HUpLockIdxBack); apply iff_refl; fail
+                   |instantiate (1:= HUpLockBackNone); apply iff_refl; fail
+                   |instantiate (1:= HDownLockMsgId _ _); apply iff_refl; fail
+                   |instantiate (1:= HDownLockMsg); apply iff_refl; fail
+                   |instantiate (1:= HDownLockIdxBack); apply iff_refl; fail
+                   |instantiate (1:= HMsgIdFrom _); apply iff_refl; fail].
+
+        instantiate (1:= HOPrecProp _); simpl.
+        instantiate (1:= HNatLe (w:= 3) _ _); simpl.
+        instantiate (2:= HBExp (HBConst _ (HBConstNat _ Mesi.mesiS))); simpl.
+        instantiate (1:= HBExp (HOstVal _ status eq_refl)); simpl.
+        setoid_rewrite <-eq_rect_eq.
+        apply iff_refl.
+
+    - intros.
+      repeat autounfold with MesiRules.
+      cbv [immDownRule].
+      cbv [rule_trs].
+
+      instantiate (1:= HTrsMTrs (HMTrs _)); simpl.
+      apply TrsMTrs_ext; intros.
+      instantiate (1:= fun var => HBind (var:= var) _ _); simpl.
+      instantiate (3:= HGetFirstMsg); simpl.
+      instantiate (1:= fun msg => HRet _ _ _).
+      simpl; repeat f_equal.
+      apply functional_extensionality; intros msg.
+      repeat f_equal.
+      { instantiate (1:= HOStateI _); reflexivity. }
+      { instantiate (1:= HORqI _); reflexivity. }
+      { instantiate (1:= HMsgOutExt _ _).
+        simpl; repeat f_equal.
+        { cbv [rsMsg miv_id miv_value].
+          instantiate (1:= HBExp (HMsgB _ _ _)).
+          simpl; f_equal.
+          { instantiate (1:= HBConst _ (HBConstIdx hcfg_msg_id_sz _)); reflexivity. }
+          { instantiate (1:= HBConst _ (HBConstBool _)); reflexivity. }
+          { instantiate (1:= HOstVal _ val eq_refl).
+            simpl; setoid_rewrite <-eq_rect_eq.
+            reflexivity.
+          }
+        }
+      }
+  Defined.
+
+End Tests.
+
